src/Formalization/Examples/Interprocedural/Example_Proc_Recursion_CFG.thy
@@ -1,0 +1,64 @@
+section \<open>Example: recursive procedure CFG layout\<close>
+
+theory Example_Proc_Recursion_CFG
+  imports "Voblint_CFG.IMP2_Proc_to_CFG" "Voblint_IMP2.IMP2_Notation"
+begin
+
+text \<open>
+  Source-level regression for procedure layout.  The procedure list is known
+  before any body is compiled, so calls may target the current procedure, a
+  later procedure, or a mutually recursive sibling.
+\<close>
+
+definition proc_layout_regression_prog :: imp_prog where
+  "proc_layout_regression_prog = \<lbrakk>
+     int G;
+     void f() {
+       if (G < 1) { f() } else { G := G }
+     }
+     void g() { h() }
+     void h() { g() }
+     void inc() { G := G + 1 }
+     void main() { f(); g(); inc() }
+   \<rbrakk>"
+
+definition proc_layout_regression_cfg :: cfg where
+  "proc_layout_regression_cfg =
+     compile_prog (prog_table proc_layout_regression_prog)
+       (prog_procs proc_layout_regression_prog)
+       (prog_main proc_layout_regression_prog)"
+
+lemma proc_layout_regression_direct_recursion:
+  "(1, EA_Enter, 0) \<in> edges proc_layout_regression_cfg \<and>
+   (1, 5, 2) \<in> combines proc_layout_regression_cfg"
+  unfolding proc_layout_regression_cfg_def proc_layout_regression_prog_def by eval
+
+lemma proc_layout_regression_mutual_recursion:
+  "(6, EA_Enter, 8) \<in> edges proc_layout_regression_cfg \<and>
+   (8, EA_Enter, 6) \<in> edges proc_layout_regression_cfg \<and>
+   (6, 9, 7) \<in> combines proc_layout_regression_cfg \<and>
+   (8, 7, 9) \<in> combines proc_layout_regression_cfg"
+  unfolding proc_layout_regression_cfg_def proc_layout_regression_prog_def by eval
+
+lemma proc_layout_regression_forward_call:
+  "(6, EA_Enter, 8) \<in> edges proc_layout_regression_cfg \<and>
+   (6, 9, 7) \<in> combines proc_layout_regression_cfg"
+  unfolding proc_layout_regression_cfg_def proc_layout_regression_prog_def by eval
+
+lemma proc_layout_regression_ordinary_call:
+  "(16, EA_Enter, 10) \<in> edges proc_layout_regression_cfg \<and>
+   (16, 11, 17) \<in> combines proc_layout_regression_cfg"
+  unfolding proc_layout_regression_cfg_def proc_layout_regression_prog_def by eval
+
+lemma proc_layout_regression_regions:
+  "compile_prog_regions (prog_table proc_layout_regression_prog)
+     (prog_procs proc_layout_regression_prog)
+     (prog_main proc_layout_regression_prog) =
+   [(None, [12, 13, 14, 15, 16, 17]),
+    (Some ''f'', [0, 1, 2, 3, 4, 5]),
+    (Some ''g'', [6, 7]),
+    (Some ''h'', [8, 9]),
+    (Some ''inc'', [10, 11])]"
+  unfolding proc_layout_regression_prog_def by eval
+
+end
